pulse/share/steel/examples/pulse/lib/Pulse.Lib.Vec.fst
@@ -6,8 +6,6 @@ open Pulse.Lib.Pervasives
 module R = Pulse.Lib.Reference
 module A = Pulse.Lib.Array.Core
 
-friend Pulse.Lib.Core
-
 type vec a = A.array a
 let length v = A.length v
 let is_full_vec v = A.is_full_array v
@@ -36,7 +34,13 @@ fn vec_ref_read' (#a:Type0) (r:R.ref (vec a)) (i:SZ.t)
   returns x:a
   ensures R.pts_to r v ** pts_to v s ** pure (x == Seq.index s (SZ.v i))
 {
-  admit ()
+  let vc = !r;
+  rewrite (pts_to (reveal v) s)
+       as (pts_to vc s);
+  let x = op_Array_Access vc i;
+  rewrite (pts_to vc s)
+       as (pts_to (reveal v) s);
+  x
 }
 ```
 
@@ -49,7 +53,13 @@ fn vec_ref_write' (#a:Type0) (r:R.ref (vec a)) (i:SZ.t) (x:a)
   requires R.pts_to r v ** pts_to v s
   ensures R.pts_to r v ** pts_to v (Seq.upd s (SZ.v i) x)
 {
-  admit ()
+  let vc = !r;
+  rewrite (pts_to (reveal v) s)
+       as (pts_to vc s);
+  op_Array_Assignment vc i x;
+  with s. assert (pts_to vc s);
+  rewrite (pts_to vc s)
+       as (pts_to (reveal v) s)
 }
 ```
 
